fix poly1305_finish

code/experimental/poly1305/Hacl.Impl.Poly1305.fst
@@ -3,6 +3,7 @@ module Hacl.Impl.Poly1305
 module ST = FStar.HyperStack.ST
 open FStar.HyperStack
 open FStar.HyperStack.All
+
 open Lib.IntTypes
 open Lib.Buffer
 open Lib.ByteBuffer
@@ -10,55 +11,71 @@ open Lib.ByteBuffer
 open Hacl.Impl.Poly1305.Fields
 
 module F32 = Hacl.Impl.Poly1305.Field32
-module F64 = Hacl.Impl.Poly1305.Field64
+//module F64 = Hacl.Impl.Poly1305.Field64
 module F128 = Hacl.Impl.Poly1305.Field128
 module F256 = Hacl.Impl.Poly1305.Field256
 
 inline_for_extraction
-val poly1305_encode_block: #s:field_spec -> f:felem s -> b:lbuffer uint8 16ul -> Stack unit
-                   (requires (fun h -> live h b /\ live h f ))
-		   (ensures (fun h0 _ h1 -> modifies (loc f) h0 h1))
-let poly1305_encode_block #s f b = 
-    load_felem_le f b;
-    set_bit128 f 
+val poly1305_encode_block:
+    #s:field_spec
+  -> f:felem s
+  -> b:lbuffer uint8 16ul
+  -> Stack unit
+    (requires fun h -> live h b /\ live h f)
+    (ensures  fun h0 _ h1 -> modifies (loc f) h0 h1)
+let poly1305_encode_block #s f b =
+  load_felem_le f b;
+  set_bit128 f
 
 inline_for_extraction
-val poly1305_encode_blocks: #s:field_spec -> f:felem s -> b:lbuffer uint8 (blocklen s) -> Stack unit
-                   (requires (fun h -> live h b /\ live h f ))
-		   (ensures (fun h0 _ h1 -> modifies (loc f) h0 h1))
-let poly1305_encode_blocks #s f b = 
-    load_felems_le f b;
-    set_bit128 f 
+val poly1305_encode_blocks:
+    #s:field_spec
+  -> f:felem s
+  -> b:lbuffer uint8 (blocklen s)
+  -> Stack unit
+    (requires fun h -> live h b /\ live h f)
+    (ensures  fun h0 _ h1 -> modifies (loc f) h0 h1)
+let poly1305_encode_blocks #s f b =
+  load_felems_le f b;
+  set_bit128 f
 
 inline_for_extraction
-val poly1305_encode_last: #s:field_spec -> f:felem s -> len:size_t{v len < 16} -> b:lbuffer uint8 len -> Stack unit
-                   (requires (fun h -> live h b /\ live h f ))
-		   (ensures (fun h0 _ h1 -> modifies (loc f) h0 h1))
+val poly1305_encode_last:
+    #s:field_spec
+  -> f:felem s
+  -> len:size_t{v len < 16}
+  -> b:lbuffer uint8 len
+  -> Stack unit
+    (requires fun h -> live h b /\ live h f)
+    (ensures  fun h0 _ h1 -> modifies (loc f) h0 h1)
 #reset-options "--z3rlimit 200"
-let poly1305_encode_last #s f len b = 
-    push_frame();
-    let tmp = create (size 16) (u8 0) in
-    copy (sub tmp 0ul len) (sub b 0ul len);
-    load_felem_le f tmp;
-    set_bit f (len *. size 8);
-    pop_frame()
+let poly1305_encode_last #s f len b =
+  push_frame();
+  let tmp = create (size 16) (u8 0) in
+  copy (sub tmp 0ul len) (sub b 0ul len);
+  load_felem_le f tmp;
+  set_bit f (len *. size 8);
+  pop_frame()
 
 inline_for_extraction
-val poly1305_encode_r: #s:field_spec -> p:precomp_r s -> b:lbuffer uint8 16ul -> Stack unit
-                   (requires (fun h -> live h b /\ live h p ))
-		   (ensures (fun h0 _ h1 -> modifies (loc p) h0 h1))
-let poly1305_encode_r #s p b = 
-    let lo = uint_from_bytes_le (sub b 0ul 8ul) in
-    let hi = uint_from_bytes_le (sub b 8ul 8ul) in
-    let mask0 = u64 0x0ffffffc0fffffff in
-    let mask1 = u64 0x0ffffffc0ffffffc in
-    let lo = lo &. mask0 in
-    let hi = hi &. mask1 in
-    load_precompute_r p lo hi
+val poly1305_encode_r:
+    #s:field_spec
+  -> p:precomp_r s
+  -> b:lbuffer uint8 16ul
+  -> Stack unit
+    (requires fun h -> live h b /\ live h p)
+    (ensures  fun h0 _ h1 -> modifies (loc p) h0 h1)
+let poly1305_encode_r #s p b =
+  let lo = uint_from_bytes_le (sub b 0ul 8ul) in
+  let hi = uint_from_bytes_le (sub b 8ul 8ul) in
+  let mask0 = u64 0x0ffffffc0fffffff in
+  let mask1 = u64 0x0ffffffc0ffffffc in
+  let lo = lo &. mask0 in
+  let hi = hi &. mask1 in
+  load_precompute_r p lo hi
 
-  
 inline_for_extraction
-type poly1305_ctx (s:field_spec) = lbuffer (limb s) (nlimb s *. 2ul +. precomplen s)
+type poly1305_ctx (s:field_spec) = lbuffer (limb s) (nlimb s +. precomplen s)
 
 (*
 inline_for_extraction
@@ -66,7 +83,7 @@ val get_acc: #s:field_spec -> ctx:poly1305_ctx s -> Stack (felem s)
                    (requires (fun h -> live h ctx))
 		   (ensures (fun h0 r h1 -> h0 == h1 /\ live h1 r))
 *)
-inline_for_extraction 
+inline_for_extraction
 let get_acc #s (ctx:poly1305_ctx s) = sub ctx (size 0) (nlimb s)
 
 
@@ -79,31 +96,20 @@ val get_precomp_r: #s:field_spec -> ctx:poly1305_ctx s -> Stack (precomp_r s)
 inline_for_extraction
 let get_precomp_r #s (ctx:poly1305_ctx s) = sub ctx (nlimb s) (precomplen s)
 
-(*
 inline_for_extraction
-val get_s: #s:field_spec -> ctx:poly1305_ctx s -> Stack (felem s)
-                   (requires (fun h -> live h ctx))
-		   (ensures (fun h0 r h1 -> h0 == h1 /\ live h1 r))
-*)
-inline_for_extraction
-let get_s #s (ctx:poly1305_ctx s) = sub ctx (nlimb s +. precomplen s) (nlimb s)
-
-
-inline_for_extraction
-val poly1305_init_: #s:field_spec -> ctx:poly1305_ctx s -> key:lbuffer uint8 32ul -> Stack unit
-                   (requires (fun h -> live h ctx /\ live h key))
-		   (ensures (fun h0 _ h1 -> modifies (loc ctx) h0 h1))
-let poly1305_init_ #s ctx key = 
+val poly1305_init_:
+    #s:field_spec
+  -> ctx:poly1305_ctx s
+  -> key:lbuffer uint8 32ul
+  -> Stack unit
+    (requires fun h -> live h ctx /\ live h key)
+    (ensures  fun h0 _ h1 -> modifies (loc ctx) h0 h1)
+let poly1305_init_ #s ctx key =
   let kr = sub key (size 0) (size 16) in
-  let ks = sub key (size 16) (size 16) in
-  
   let acc = get_acc ctx in
   let precomp_r = get_precomp_r ctx in
-  let sk = get_s ctx in 
   set_zero acc;
-  poly1305_encode_r precomp_r kr;
-  load_felem_le sk ks;
-  admit()
+  poly1305_encode_r precomp_r kr
 
 (* WRAPPER TO PREVENT INLINING *)
 [@CInline]
@@ -114,46 +120,59 @@ inline_for_extraction
 let poly1305_init_256 (ctx:poly1305_ctx M256) (k:lbuffer uint8 32ul) = poly1305_init_ #M256 ctx k
 
 inline_for_extraction noextract
-val poly1305_init: #s:field_spec -> ctx:poly1305_ctx s -> key:lbuffer uint8 32ul -> Stack unit
-                   (requires (fun h -> live h ctx /\ live h key))
-		   (ensures (fun h0 _ h1 -> modifies (loc ctx) h0 h1))
-let poly1305_init #s ctx key = 
-   match s with
-   | M32 -> poly1305_init_32 ctx key
-   | M128 -> poly1305_init_128 ctx key
-   | M256 -> poly1305_init_256 ctx key
+val poly1305_init:
+    #s:field_spec
+  -> ctx:poly1305_ctx s
+  -> key:lbuffer uint8 32ul
+  -> Stack unit
+    (requires fun h -> live h ctx /\ live h key)
+    (ensures  fun h0 _ h1 -> modifies (loc ctx) h0 h1)
+let poly1305_init #s ctx key =
+  match s with
+  | M32 -> poly1305_init_32 ctx key
+  | M128 -> poly1305_init_128 ctx key
+  | M256 -> poly1305_init_256 ctx key
 (* WRAPPER to Prevent Inlining *)
 
 
 
 inline_for_extraction
-val poly1305_nblocks: #s:field_spec -> ctx:poly1305_ctx s -> len:size_t{v len % v (blocklen s) == 0}  -> text:lbuffer uint8 len -> Stack unit
-                   (requires (fun h -> live h ctx /\ live h text))
-		   (ensures (fun h0 _ h1 -> modifies (loc ctx) h0 h1))
-
-let poly1305_nblocks #s ctx len text = 
+val poly1305_nblocks:
+    #s:field_spec
+  -> ctx:poly1305_ctx s
+  -> len:size_t{v len % v (blocklen s) == 0}
+  -> text:lbuffer uint8 len
+  -> Stack unit
+    (requires fun h -> live h ctx /\ live h text)
+    (ensures  fun h0 _ h1 -> modifies (loc ctx) h0 h1)
+let poly1305_nblocks #s ctx len text =
   push_frame();
   let acc = get_acc ctx in
   let pre = get_precomp_r ctx in
   let e = create (nlimb s) (limb_zero s) in
   let sz_block = blocklen s in
-  let blocks = len /. sz_block  in
+  let blocks = len /. sz_block in
   let h0 = ST.get() in
   admit();
-  loop_nospec #h0 blocks ctx 
-    (fun i ->
-       let b = sub text (i *. sz_block) sz_block in
-       poly1305_encode_blocks e b;
-       fmul_rn acc acc pre;
-       fadd acc acc e);
+  loop_nospec #h0 blocks ctx
+  (fun i ->
+    let b = sub text (i *. sz_block) sz_block in
+    poly1305_encode_blocks e b;
+    fmul_rn acc acc pre;
+    fadd acc acc e
+  );
   fmul_rn_normalize acc pre;
   pop_frame()
 
 inline_for_extraction
-val poly1305_update_: #s:field_spec -> ctx:poly1305_ctx s -> len:size_t -> text:lbuffer uint8 len -> Stack unit
-                   (requires (fun h -> live h ctx /\ live h text))
-		   (ensures (fun h0 _ h1 -> modifies (loc ctx) h0 h1))
-
+val poly1305_update_:
+    #s:field_spec
+  -> ctx:poly1305_ctx s
+  -> len:size_t
+  -> text:lbuffer uint8 len
+  -> Stack unit
+    (requires fun h -> live h ctx /\ live h text)
+    (ensures  fun h0 _ h1 -> modifies (loc ctx) h0 h1)
 let poly1305_update_ #s ctx len text =
   push_frame();
   let acc = get_acc ctx in
@@ -170,16 +189,17 @@ let poly1305_update_ #s ctx len text =
   let blocks = len /. size 16 in
   let h0 = ST.get() in
   admit();
-  loop_nospec #h0 blocks ctx 
-    (fun i ->
-       let b = sub text (i *. size 16) (size 16) in
-       poly1305_encode_block e b;
-       fadd_mul_r acc e pre);
+  loop_nospec #h0 blocks ctx
+  (fun i ->
+    let b = sub text (i *. size 16) (size 16) in
+    poly1305_encode_block e b;
+    fadd_mul_r acc e pre
+  );
   let rem = len %. size 16 in
   if (rem >. size 0) then (
-     let b = sub text (blocks *. size 16) rem in
-     poly1305_encode_last e rem b;
-     fadd_mul_r acc e pre);
+    let b = sub text (blocks *. size 16) rem in
+    poly1305_encode_last e rem b;
+    fadd_mul_r acc e pre);
   pop_frame()
 
 (* WRAPPER TO PREVENT INLINING *)
@@ -191,60 +211,85 @@ inline_for_extraction
 let poly1305_update_256 (ctx:poly1305_ctx M256) (len:size_t) (text:lbuffer uint8 len) = poly1305_update_ #M256 ctx len text
 
 inline_for_extraction noextract
-val poly1305_update: #s:field_spec -> ctx:poly1305_ctx s -> len:size_t -> text:lbuffer uint8 len -> Stack unit
-                   (requires (fun h -> live h ctx /\ live h text))
-		   (ensures (fun h0 _ h1 -> modifies (loc ctx) h0 h1))
-let poly1305_update #s ctx len text = 
-   match s with
-   | M32 -> poly1305_update_32 ctx len text
-   | M128 -> poly1305_update_128 ctx len text
-   | M256 -> poly1305_update_256 ctx len text
+val poly1305_update:
+    #s:field_spec
+  -> ctx:poly1305_ctx s
+  -> len:size_t
+  -> text:lbuffer uint8 len
+  -> Stack unit
+    (requires fun h -> live h ctx /\ live h text)
+    (ensures  fun h0 _ h1 -> modifies (loc ctx) h0 h1)
+let poly1305_update #s ctx len text =
+  match s with
+  | M32 -> poly1305_update_32 ctx len text
+  | M128 -> poly1305_update_128 ctx len text
+  | M256 -> poly1305_update_256 ctx len text
 (* WRAPPER to Prevent Inlining *)
 
 
 inline_for_extraction
-val poly1305_finish_: #s:field_spec -> ctx:poly1305_ctx s -> tag:lbuffer uint8 16ul -> Stack unit 
-		     (requires (fun h -> live h ctx /\ live h tag))
-		     (ensures (fun h0 _ h1 -> modifies (loc tag) h0 h1))
-		  
-let poly1305_finish_ #s ctx tag = 
+val poly1305_finish_:
+    #s:field_spec
+  -> key:lbuffer uint8 32ul
+  -> ctx:poly1305_ctx s
+  -> tag:lbuffer uint8 16ul
+  -> Stack unit
+    (requires fun h -> live h ctx /\ live h tag /\ live h key)
+    (ensures  fun h0 _ h1 -> modifies (loc tag) h0 h1)
+let poly1305_finish_ #s key ctx tag = admit();
+  push_frame ();
   let acc = get_acc ctx in
-  let sk = get_s ctx in
   reduce_felem acc;
+
+  let ks = sub key (size 16) (size 16) in
+  let sk = create (nlimb s) (limb_zero s) in
+  load_felem_le sk ks;
+
+  //use u128 addition
   fadd acc acc sk;
   store_felem_le tag acc;
-  admit()
+  pop_frame ()
 
 (* WRAPPER TO PREVENT INLINING *)
 [@CInline]
-let poly1305_finish_32 (ctx:poly1305_ctx M32) (tag:lbuffer uint8 16ul) = poly1305_finish_ #M32 ctx tag
+let poly1305_finish_32 (key:lbuffer uint8 32ul) (ctx:poly1305_ctx M32) (tag:lbuffer uint8 16ul) = poly1305_finish_ #M32 key ctx tag
 [@CInline]
-let poly1305_finish_128 (ctx:poly1305_ctx M128) (tag:lbuffer uint8 16ul) = poly1305_finish_ #M128 ctx tag
+let poly1305_finish_128 (key:lbuffer uint8 32ul) (ctx:poly1305_ctx M128) (tag:lbuffer uint8 16ul) = poly1305_finish_ #M128 key ctx tag
 [@CInline]
-let poly1305_finish_256 (ctx:poly1305_ctx M256) (tag:lbuffer uint8 16ul) = poly1305_finish_ #M256 ctx tag
+let poly1305_finish_256 (key:lbuffer uint8 32ul) (ctx:poly1305_ctx M256) (tag:lbuffer uint8 16ul) = poly1305_finish_ #M256 key ctx tag
 
 inline_for_extraction noextract
-val poly1305_finish: #s:field_spec -> ctx:poly1305_ctx s -> tag:lbuffer uint8 16ul -> Stack unit 
-		     (requires (fun h -> live h ctx /\ live h tag))
-		     (ensures (fun h0 _ h1 -> modifies (loc tag) h0 h1))
-let poly1305_finish #s ctx tag = 
+val poly1305_finish:
+    #s:field_spec
+  -> key:lbuffer uint8 32ul
+  -> ctx:poly1305_ctx s
+  -> tag:lbuffer uint8 16ul
+  -> Stack unit
+    (requires fun h -> live h ctx /\ live h tag /\ live h key)
+    (ensures  fun h0 _ h1 -> modifies (loc tag) h0 h1)
+let poly1305_finish #s key ctx tag =
    match s with
-   | M32 -> poly1305_finish_32 ctx tag
-   | M128 -> poly1305_finish_128 ctx tag
-   | M256 -> poly1305_finish_256 ctx tag
+   | M32 -> poly1305_finish_32 key ctx tag
+   | M128 -> poly1305_finish_128 key ctx tag
+   | M256 -> poly1305_finish_256 key ctx tag
 (* WRAPPER to Prevent Inlining *)
 
 
 
 inline_for_extraction
-val poly1305_mac: #s:field_spec -> tag:lbuffer uint8 16ul -> len:size_t -> text:lbuffer uint8 len ->  key:lbuffer uint8 32ul -> Stack unit 
-		     (requires (fun h -> live h text /\ live h tag /\ live h key))
- 		     (ensures (fun h0 _ h1 -> modifies (loc tag) h0 h1))
-let poly1305_mac #s tag len text key = 
-  push_frame();
-  let ctx = create (nlimb s *. 2ul +. precomplen s) (limb_zero s) in
+val poly1305_mac:
+    #s:field_spec
+  -> tag:lbuffer uint8 16ul
+  -> len:size_t
+  -> text:lbuffer uint8 len
+  -> key:lbuffer uint8 32ul
+  -> Stack unit
+    (requires fun h -> live h text /\ live h tag /\ live h key)
+    (ensures  fun h0 _ h1 -> modifies (loc tag) h0 h1)
+let poly1305_mac #s tag len text key =
+  push_frame ();
+  let ctx = create (nlimb s +. precomplen s) (limb_zero s) in
   poly1305_init ctx key;
   poly1305_update ctx len text;
-  poly1305_finish ctx tag;
-  pop_frame()
-
+  poly1305_finish key ctx tag;
+  pop_frame ()
